Initial round of testing works with new syntax.  Fixed an error where floating points could not be given as a function argument

Source/Core/Parser.cs
@@ -668,9 +668,8 @@ private class BvBounds : Expr {
    ty = new BasicType(t, SimpleType.Real);
   } else if (la.kind == 98) {
    Get();
-   if (la.kind == 3) {
-     Get();
-    switch (Int32.Parse(t.val)) {
+   if (t.val.Length > 5) {
+    switch (Int32.Parse(t.val.Substring(5))) {
     case 16:
         ty = new FloatType(t, 5, 11);
         break;
@@ -690,10 +689,10 @@ private class BvBounds : Expr {
    }
    else {
     Expect(19); //<
-    Expect(3);
+    Expect(3); //int
     int exp = Int32.Parse(t.val);
     Expect(12); //,
-    Expect(3);
+    Expect(3); //int
     int man = Int32.Parse(t.val);
     ty = new FloatType(t, exp, man);
     Expect(20); //>
@@ -1830,14 +1829,14 @@ out List<Variable>/*!*/ ins, out List<Variable>/*!*/ outs, out QKeyValue kv) {
 			break;
 		}
   case 98: {
-      Get();
-      x = t;
-      Expect(19);
-      Expression(out e);
-      Expect(20);
-      e = new NAryExpr(x, new ArithmeticCoercion(x, ArithmeticCoercion.CoercionType.ToFloat), new List<Expr> { e });
-      break;
-    }
+   Get();
+   x = t;
+   Expect(19);
+   Expression(out e);
+   Expect(20);
+   e = new NAryExpr(x, new ArithmeticCoercion(x, ArithmeticCoercion.CoercionType.ToFloat), new List<Expr> { e });
+   break;
+  }
 		case 9: {
 			Get();
 			if (StartOf(9)) {
@@ -2188,7 +2187,7 @@ out QKeyValue kv, out Trigger trig, out Expr/*!*/ body) {
 	static readonly bool[,]/*!*/ set = { //grid is 17 x 100
 		{T,x,x,x, x,x,x,x, x,x,x,x, x,x,x,x, x,x,x,x, x,x,x,x, x,x,x,x, x,x,x,x, x,x,x,x, x,x,x,x, x,x,x,x, x,x,x,x, x,x,x,x, x,x,x,x, x,x,x,x, x,x,x,x, x,x,x,x, x,x,x,x, x,x,x,x, x,x,x,x, x,x,x,x, x,x,x,x, x,x,x,x, x,x,x,x, x,x,x,x},
 		{x,x,x,x, x,x,x,T, x,x,x,x, x,x,x,x, x,x,x,x, x,T,x,x, x,T,x,x, x,T,T,x, T,T,x,x, x,x,x,x, x,x,x,x, x,x,x,x, x,x,x,x, x,x,x,x, x,x,x,x, x,x,x,x, x,x,x,x, x,x,x,x, x,x,x,x, x,x,x,x, x,x,x,x, x,x,x,x, x,x,x,x, x,x,x,x, x,x,x,x},
-		{x,T,x,x, x,x,x,x, x,T,x,x, x,x,T,T, T,T,x,T, x,x,x,x, x,x,x,T, x,x,x,x, x,x,x,x, x,x,x,x, x,x,x,x, x,x,x,x, x,x,x,x, x,x,x,x, x,x,x,x, x,x,x,x, x,x,x,x, x,x,x,x, x,x,x,x, x,x,x,x, x,x,x,x, x,x,x,x, x,x,x,x, x,x,x,x, x,x,x,x},
+		{x,T,x,x, x,x,x,x, x,T,x,x, x,x,T,T, T,T,x,T, x,x,x,x, x,x,x,T, x,x,x,x, x,x,x,x, x,x,x,x, x,x,x,x, x,x,x,x, x,x,x,x, x,x,x,x, x,x,x,x, x,x,x,x, x,x,x,x, x,x,x,x, x,x,x,x, x,x,x,x, x,x,x,x, x,x,x,x, x,x,x,x, x,x,x,x, x,x,T,x},
 		{x,x,x,x, x,x,x,x, x,x,x,x, x,x,x,x, x,x,x,x, x,x,x,x, x,x,x,x, x,x,x,x, x,x,T,T, T,T,x,x, x,x,x,x, x,x,x,x, x,x,x,x, x,x,x,x, x,x,x,x, x,x,x,x, x,x,x,x, x,x,x,x, x,x,x,x, x,x,x,x, x,x,x,x, x,x,x,x, x,x,x,x, x,x,x,x, x,x,x,x},
 		{x,x,x,x, x,x,x,x, x,x,x,x, x,x,x,x, x,x,x,x, x,x,x,x, x,x,x,T, x,x,x,x, x,x,T,T, T,T,x,x, x,x,x,x, x,x,x,x, x,x,x,x, x,x,x,x, x,x,x,x, x,x,x,x, x,x,x,x, x,x,x,x, x,x,x,x, x,x,x,x, x,x,x,x, x,x,x,x, x,x,x,x, x,x,x,x, x,x,x,x},
 		{x,x,x,x, x,x,x,x, x,T,x,x, x,x,T,T, T,x,x,x, x,x,x,x, x,x,x,x, x,x,x,x, x,x,x,x, x,x,x,x, x,x,x,x, x,x,x,x, x,x,x,x, x,x,x,x, x,x,x,x, x,x,x,x, x,x,x,x, x,x,x,x, x,x,x,x, x,x,x,x, x,x,x,x, x,x,x,x, x,x,x,x, x,x,x,x, x,x,T,x},
