float_test11.bpl
@@ -1,38 +1,55 @@
 //Translation from interpolation.c
 //Should Verify
-//Returns inconclusize?  What does that mean?
+//Returns inconclusive?  What does that mean?
 
+function {:builtin "(_ to_fp 8 24) RNE"} TO_FLOAT32_INT(int) returns (float32);
 procedure main() returns () {
 	var i : int;
-	var z : float;
-	var t : float;
-	var min : [int] float;
-	var max : [int] float;
+	var z : float32;
+	var t : float32;
+	var min : [int] float32;
+	var max : [int] float32;
 	
-	min[0] := fp(5);
-	min[1] := fp(10);
-	min[2] := fp(12);
-	min[3] := fp(30);
-	min[4] := fp(150);
+	min[0] := TO_FLOAT32_INT(5);
+	min[1] := TO_FLOAT32_INT(10);
+	min[2] := TO_FLOAT32_INT(12);
+	min[3] := TO_FLOAT32_INT(30);
+	min[4] := TO_FLOAT32_INT(150);
 	
-	max[0] := fp(10);
-	max[1] := fp(12);
-	max[2] := fp(30);
-	max[3] := fp(150);
-	max[4] := fp(300);
+	max[0] := TO_FLOAT32_INT(10);
+	max[1] := TO_FLOAT32_INT(12);
+	max[2] := TO_FLOAT32_INT(30);
+	max[3] := TO_FLOAT32_INT(150);
+	max[4] := TO_FLOAT32_INT(300);
 	
 	havoc t;
 	assume(t >= min[0] && t <= max[4]);
 	
 	i := 0;
-	while (i < 5) {
-		if (t <= max[i]) {
-			break;
-		}
+	//while (i < 5) {
+		//if (t <= max[i]) {
+			//break;
+		//}
+		//i := i + 1;
+	//}
+	
+	if (t > max[0]) { //1
+		i := i + 1;
+	}
+	if (t > max[1]) { //2
+		i := i + 1;
+	}
+	if (t > max[2]) { //3
+		i := i + 1;
+	}
+	if (t > max[3]) { //4
+		i := i + 1;
+	}
+	if (t > max[4]) { //5
 		i := i + 1;
 	}
 	
 	z := (t - min[i]) / (max[i] - min[i]);
 	
-	assert(z >= fp(0) && z <= fp(1));
+	assert(z >= TO_FLOAT32_INT(0) && z <= TO_FLOAT32_INT(1));
 }
