float_test13.bpl
@@ -1,17 +1,19 @@
 //Translation from inv_square_false-unreach-call.c
 //Should return an error (without crashing)
 
+function {:builtin "(_ to_fp 8 24) RNE"} TO_FLOAT32_INT(int) returns (float32);
+
 procedure main() returns () {
-	var x : float;
-	var y : float;
-	var z : float;
+	var x : float32;
+	var y : float32;
+	var z : float32;
 	
 	havoc x;
-	assume(x >= fp(-1) && x <= fp(1));
+	assume(x >= TO_FLOAT32_INT(-1) && x <= TO_FLOAT32_INT(1));
 	
-	if (x != fp(0)) {
+	if (x != TO_FLOAT32_INT(0)) {
 		y := x * x;
-		assert(y != fp(0));
-		z := fp(1) / y;
+		assert(y != TO_FLOAT32_INT(0));
+		z := TO_FLOAT32_INT(1) / y;
 	}
 }
