float_test14.bpl
@@ -1,17 +1,20 @@
-//Translation from inv_square_false-unreach-call.c
+//Translation from inv_square_true-unreach-call.c
 //Should Verify
 
+function {:builtin "(_ to_fp 8 24) RNE"} TO_FLOAT32_INT(int) returns (float32);
+function {:builtin "(_ to_fp 8 24) RNE"} TO_FLOAT32_REAL(real) returns (float32);
+
 procedure main() returns () {
-	var x : float;
-	var y : float;
-	var z : float;
+	var x : float32;
+	var y : float32;
+	var z : float32;
 	
 	havoc x;
-	assume(x >= fp(-1) && x <= fp(1));
+	assume(x >= TO_FLOAT32_INT(-1) && x <= TO_FLOAT32_INT(1));
 	
-	if (x <= fp(-.00000000000000000001) || x >= fp(.00000000000000000001)) {
+	if (x <= TO_FLOAT32_REAL(-1e-20) || x >= TO_FLOAT32_REAL(1e-20)) {
 		y := x * x;
-		assert(y != fp(0));
-		z := fp(1) / y;
+		assert(y != TO_FLOAT32_INT(0));
+		z := TO_FLOAT32_INT(1) / y;
 	}
 }
