float_test2.bpl
@@ -1,13 +1,17 @@
 //Translation from addsub_float_exact.c
 //Should Verify
+
+function {:builtin "(_ to_fp 8 24) RNE"} TO_FLOAT32_INT(int) returns (float32);
+function {:builtin "(_ to_fp 8 24) RNE"} TO_FLOAT32_REAL(real) returns (float32);
+
 procedure main() returns () {
-	var x : float;
-	var y : float;
-	var z : float;
-	var r : float;
-	x := fp(1000000);
-	y := x + fp(1);
-	z := x - fp(1);
+	var x : float32;
+	var y : float32;
+	var z : float32;
+	var r : float32;
+	x := TO_FLOAT32_REAL(1e7);
+	y := x + TO_FLOAT32_INT(1);
+	z := x - TO_FLOAT32_INT(1);
 	r := y - z;
-	assert r == fp(2);
+	assert r == TO_FLOAT32_INT(2);
 }
