float_test8.bpl
@@ -1,12 +1,16 @@
 //Translation from float_double.c
 //Should Verify
-//FAILS: I don't have this functionality yet...
+
+function {:builtin "(_ to_fp 11 53) RNE"} TO_FLOAT64_FLOAT32(float32) returns (float64);
+function {:builtin "(_ to_fp 8 24) RNE"} TO_FLOAT32_FLOAT64(float64) returns (float32);
+function {:builtin "(_ to_fp 11 53) RNE"} TO_FLOAT64_INT(int) returns (float64);
+function {:builtin "(_ to_fp 11 53) RNE"} TO_FLOAT64_REAL(real) returns (float64);
 
 procedure main() returns () {
-	var x : float(11 53);
-	var y : float;
+	var x : float64;
+	var y : float32;
 	
-	x := fp(100000000000000000001 11 53);
-	y := x;
-	assert(x != y);
+	x := TO_FLOAT64_REAL(1e20)+TO_FLOAT64_INT(1);
+	y := TO_FLOAT32_FLOAT64(x);
+	assert x != TO_FLOAT64_FLOAT32(y);
 }
