float_test3.bpl
@@ -1,13 +1,13 @@
 //Translation from addsub_float_inexact.c
 //Should give an error
 procedure main() returns () {
-	var x : float;
-	var y : float;
-	var z : float;
-	var r : float;
-	x := fp(10000000);
-	y := x + fp(1);
-	z := x - fp(1);
+	var x : float32;
+	var y : float32;
+	var z : float32;
+	var r : float32;
+	x := fp<8, 24>(3221225472bv32);
+	y := x + fp<8, 24>(1bv32);
+	z := x - fp<8, 24>(1bv32);
 	r := y - z;
-	assert r == fp(0);
+	assert r == fp<8, 24>(2bv32);
 }
