float_test5.bpl
@@ -1,15 +1,18 @@
 //Translation from filter1.c
 //Should Verify
 
+function {:builtin "(_ to_fp 11 53) RNE"} TO_FLOAT64_INT(int) returns (float64);
+function {:builtin "(_ to_fp 11 53) RNE"} TO_FLOAT64_REAL(real) returns (float64);
+
 procedure main() returns () {
-	var E0 : float(11 53);
-	var E1 : float(11 53);
-	var S : float(11 53);
+	var E0 : float64;
+	var E1 : float64;
+	var S : float64);
 	var i : int;
 	var rand : int;
 	
-	E1 := fp(0 11 53);
-	S := fp(0 11 53);
+	E1 := TO_FLOAT64_INT(0);
+	S := TO_FLOAT64_INT(0);
 	
 	i := 0;
 	while (i <= 1000000)
